Replace nf and neutrals by their strong variant everywhere.

theories/UntypedValues.v
@@ -1,5 +1,5 @@
 From LogRel.AutoSubst Require Import core unscoped Ast Extra.
-From LogRel Require Import Utils BasicAst Notations Context UntypedReduction.
+From LogRel Require Import Utils BasicAst Notations Context Untyped UntypedReduction.
 
 Inductive snf (r : term) : Type :=
   | snf_tSort {s} : [ r ⇒* tSort s ] -> snf r
@@ -9,3 +9,96 @@ Inductive snf (r : term) : Type :=
 with sne (r : term) : Type :=
   | sne_tRel {v} : r = tRel v -> sne r
   | sne_tApp {n t} : r = tApp n t -> sne n -> snf t -> sne r.
+
+Lemma sne_whne : forall (t : term), sne t -> whne t.
+Proof.
+intros t Ht; induction Ht; subst; constructor; assumption.
+Qed.
+
+Lemma snf_red : forall t u, [ t ⇒* u ] -> snf u -> snf t.
+Proof.
+intros t u Hr Hu; destruct Hu.
++ eapply snf_tSort.
+  transitivity u; eassumption.
++ eapply snf_tProd.
+  - transitivity u; eassumption.
+  - assumption.
+  - assumption.
++ eapply snf_tLambda.
+  - transitivity u; eassumption.
+  - assumption.
+  - assumption.
++ eapply snf_sne.
+  - transitivity u; eassumption.
+  - eassumption.
+Qed.
+
+Inductive isSNType : term -> Type :=
+  | UnivType {s} : isSNType (tSort s)
+  | ProdType {na A B} : snf A -> snf B -> isSNType (tProd na A B)
+  | NeType {A}  : sne A -> isSNType A.
+
+Inductive isSNFun : term -> Type :=
+  | LamFun {na A t} : snf A -> snf t -> isSNFun (tLambda na A t)
+  | NeFun  {f} : sne f -> isSNFun f.
+
+Lemma isSNType_snf t : isSNType t -> snf t.
+Proof.
+destruct 1.
++ eapply snf_tSort; reflexivity.
++ eapply snf_tProd; first[reflexivity|assumption].
++ eapply snf_sne; first[reflexivity|assumption].
+Qed.
+
+Lemma isSNType_whnf t : isSNType t -> whnf t.
+Proof.
+destruct 1; constructor.
+apply sne_whne; assumption.
+Qed.
+
+Lemma isSNFun_snf t : isSNFun t -> snf t.
+Proof.
+destruct 1.
++ eapply snf_tLambda; first[reflexivity|assumption].
++ eapply snf_sne; first[reflexivity|assumption].
+Qed.
+
+Lemma isSNFun_whnf t : isSNFun t -> whnf t.
+Proof.
+destruct 1; constructor.
+apply sne_whne; assumption.
+Qed.
+
+Lemma isSNType_isType t : isSNType t -> isType t.
+Proof.
+destruct 1; constructor; now apply sne_whne.
+Qed.
+
+Lemma isSNFun_isFun t : isSNFun t -> isFun t.
+Proof.
+destruct 1; constructor; now apply sne_whne.
+Qed.
+
+Section RenSnf.
+
+  Variable (ρ : nat -> nat).
+
+  Lemma sne_ren t : sne t -> sne (t⟨ρ⟩).
+  Proof.
+  Admitted. (* FIXME *)
+
+  Lemma snf_ren t : snf t -> snf (t⟨ρ⟩).
+  Proof.
+  Admitted. (* FIXME *)
+
+End RenSnf.
+
+Lemma isSNType_ren ρ t : isSNType t -> isSNType (t⟨ρ⟩).
+Proof.
+destruct 1; cbn; constructor; first [apply sne_ren|apply snf_ren]; assumption.
+Qed.
+
+Lemma isSNFun_ren ρ t : isSNFun t -> isSNFun (t⟨ρ⟩).
+Proof.
+destruct 1; cbn; constructor; first [apply sne_ren|apply snf_ren]; assumption.
+Qed.
