theories/LogicalRelation/Induction.v
@@ -1,5 +1,5 @@
 From LogRel.AutoSubst Require Import core unscoped Ast Extra.
-From LogRel Require Import Utils BasicAst Notations Context Untyped Weakening GenericTyping LogicalRelation.
+From LogRel Require Import Utils BasicAst Notations Context Untyped UntypedValues Weakening GenericTyping LogicalRelation.
 
 Set Universe Polymorphism.
 
@@ -300,6 +300,7 @@ Section Inversions.
     + intros * h whA.
       epose proof (redtywf_whnf (URedTy.red h) whA); subst; assumption.
     + intros * h whA. pose (h' := h); destruct h' as [ty [?? r] ne].
+      apply sne_whne in ne.
       pose proof (redty_whnf r whA); subst.
       destruct ty; inversion ne; eassumption.
     + intros ??? h _ _ whA. pose (h' := h); destruct h' as [??? [?? r]].
